More pmap stuffs

shift-reset/gmap.v
@@ -1,5 +1,45 @@
-Module Type PositiveIsoType.
-End PositiveIsoType.
+From Stdlib Require Import PArith.
+From shift_reset Require pmap.
 
-Module Make (T : PositiveIsoType).
+Module Type IsoPositiveType.
+  Parameter t : Type.
+  Parameter encode : t -> positive.
+  Parameter decode : positive -> t.
+  Axiom decode_encode : forall (x : t), decode (encode x) = x.
+  Axiom encode_decode : forall (x : positive), encode (decode x) = x.
+End IsoPositiveType.
+
+Module Make (K : IsoPositiveType).
+  Definition key : Type := K.t.
+  Record gmap (A : Type) := GMap { gmap_car : pmap.pmap A }.
+  Definition t : Type -> Type := gmap.
+
+  Arguments GMap {A} _.
+  Arguments gmap_car {A} _.
+
+  Definition empty {A} : gmap A := GMap pmap.empty.
+
+  Definition lookup {A} (k : key) (mt : t A) : option A :=
+    pmap.lookup (K.encode k) (gmap_car mt).
+
+  Definition member {A} (k : key) (mt : t A) : bool :=
+    pmap.member (K.encode k) (gmap_car mt).
+
+  Definition singleton {A} (k : key) (x : A) : t A :=
+    GMap (pmap.singleton (K.encode k) x).
+
+  Definition insert {A} (k : key) (x : A) (mt : t A) : t A :=
+    GMap (pmap.insert (K.encode k) x (gmap_car mt)).
+
+  Definition remove {A} (k : key) (mt : t A) : t A :=
+    GMap (pmap.remove (K.encode k) (gmap_car mt)).
+
+  Definition alter {A} (f : option A -> option A) (k : key) (mt : t A) : t A :=
+    GMap (pmap.alter f (K.encode k) (gmap_car mt)).
+
+  Definition map {A B} (f : A -> B) (mt : t A) : t B :=
+    GMap (pmap.map f (gmap_car mt)).
+
+  Definition filter_map {A B} (f : A -> option B) (mt : t A) : t B :=
+    GMap (pmap.filter_map f (gmap_car mt)).
 End Make.
