shift-reset/option.v
@@ -1,0 +1,5 @@
+Definition bind {A B} (o : option A) (f : A -> option B) : option B :=
+  match o with
+  | None => None
+  | Some x => f x
+  end.
