shift-reset/pmap.v
@@ -1,7 +1,7 @@
 From Stdlib Require Import PArith.
+From shift_reset Require option.
 
 Local Open Scope positive_scope.
-
 Local Unset Elimination Schemes.
 Local Unset Case Analysis Schemes.
 
@@ -41,7 +41,7 @@ Definition PNode {A} (ml : pmap A) (mx : option A) (mr : pmap A) : pmap A :=
   | PNodes l, Some x, PNodes r => PNodes (PNode111 l x r)
   end.
 
-Definition ne_case {A B} (t : pmap_ne A) (f : pmap A -> option A -> pmap A -> B) : B :=
+Definition pmap_ne_case {A B} (t : pmap_ne A) (f : pmap A -> option A -> pmap A -> B) : B :=
   match t with
   | PNode001 r => f PEmpty None (PNodes r)
   | PNode010 x => f PEmpty (Some x) PEmpty
@@ -68,15 +68,102 @@ Definition lookup {A} (i : positive) (mt : pmap A) : option A :=
   | PNodes t => ne_lookup i t
   end.
 
-Fixpoint ne_singleton {A} (i : positive) (x : A) : pmap_ne A :=
-  match i with
-  | 1 => PNode010 x
-  | i~0 => PNode100 (ne_singleton i x)
-  | i~1 => PNode001 (ne_singleton i x)
+Fixpoint ne_member {A} (i : positive) (t : pmap_ne A) {struct t} : bool :=
+  match t, i with
+  | (PNode010 _ | PNode011 _ _ | PNode110 _ _ | PNode111 _ _ _), 1 => true
+  | (PNode100 l | PNode110 l _ | PNode101 l _ | PNode111 l _ _), i~0 => ne_member i l
+  | (PNode001 r | PNode011 _ r | PNode101 _ r | PNode111 _ _ r), i~1 => ne_member i r
+  | _, _ => false
   end.
+
+Definition member {A} (i : positive) (mt : pmap A) : bool :=
+  match mt with
+  | PEmpty => false
+  | PNodes t => ne_member i t
+  end.
+
+Definition ne_singleton {A} (i : positive) (x : A) : pmap_ne A :=
+  let fix go i :=
+    match i with
+    | 1 => PNode010 x
+    | i~0 => PNode100 (go i)
+    | i~1 => PNode001 (go i)
+    end
+  in go i.
 
 Definition singleton {A} (i : positive) (x : A) : pmap A :=
   PNodes (ne_singleton i x).
+
+Definition ne_insert {A} (i : positive) (x : A) : pmap_ne A -> pmap_ne A :=
+  let fix go i t {struct t} :=
+    match t with
+    | PNode001 r =>
+        match i with
+        | 1 => PNode011 x r
+        | i~0 => PNode101 (ne_singleton i x) r
+        | i~1 => PNode001 (go i r)
+        end
+    | PNode010 y =>
+        match i with
+        | 1 => PNode010 x
+        | i~0 => PNode110 (ne_singleton i x) y
+        | i~1 => PNode011 y (ne_singleton i x)
+        end
+    | PNode011 y r =>
+        match i with
+        | 1 => PNode011 x r
+        | i~0 => PNode111 (ne_singleton i x) y r
+        | i~1 => PNode011 y (go i r)
+        end
+    | PNode100 l =>
+        match i with
+        | 1 => PNode110 l x
+        | i~0 => PNode100 (go i l)
+        | i~1 => PNode101 l (ne_singleton i x)
+        end
+    | PNode101 l r =>
+        match i with
+        | 1 => PNode111 l x r
+        | i~0 => PNode101 (go i l) r
+        | i~1 => PNode101 l (go i r)
+        end
+    | PNode110 l y =>
+        match i with
+        | 1 => PNode110 l x
+        | i~0 => PNode110 (go i l) y
+        | i~1 => PNode111 l y (ne_singleton i x)
+        end
+    | PNode111 l y r =>
+        match i with
+        | 1 => PNode111 l x r
+        | i~0 => PNode111 (go i l) y r
+        | i~1 => PNode111 l y (go i r)
+        end
+    end
+  in go i.
+
+Definition insert {A} (i : positive) (x : A) (mt : pmap A) : pmap A :=
+  match mt with
+  | PEmpty => singleton i x
+  | PNodes t => PNodes (ne_insert i x t)
+  end.
+
+Definition remove_aux {A} (go : positive -> pmap_ne A -> pmap A) (i : positive) (mt : pmap A) : pmap A :=
+  match mt with
+  | PEmpty => PEmpty
+  | PNodes t => go i t
+  end.
+
+Fixpoint ne_remove {A} (i : positive) (t : pmap_ne A) {struct t} : pmap A :=
+  pmap_ne_case t
+    (fun ml mx mr => match i with
+                     | 1 => PNode ml None mr
+                     | i~0 => PNode (remove_aux ne_remove i ml) mx mr
+                     | i~1 => PNode ml mx (remove_aux ne_remove i mr)
+                     end).
+
+Definition remove {A} : positive -> pmap A -> pmap A :=
+  remove_aux ne_remove.
 
 Definition alter_aux {A} (go : positive -> pmap_ne A -> pmap A) (f : option A -> option A) (i : positive) (mt : pmap A) : pmap A :=
   match mt with
@@ -89,11 +176,47 @@ Definition alter_aux {A} (go : positive -> pmap_ne A -> pmap A) (f : option A ->
 
 Definition ne_alter {A} (f : option A -> option A) : positive -> pmap_ne A -> pmap A :=
   fix go i t {struct t} :=
-    ne_case t (fun ml mx mr => match i with
-                               | 1 => PNode ml (f mx) mr
-                               | i~0 => PNode (alter_aux go f i ml) mx mr
-                               | i~1 => PNode ml mx (alter_aux go f i mr)
-                               end).
+    pmap_ne_case t
+      (fun ml mx mr => match i with
+                       | 1 => PNode ml (f mx) mr
+                       | i~0 => PNode (alter_aux go f i ml) mx mr
+                       | i~1 => PNode ml mx (alter_aux go f i mr)
+                       end).
 
 Definition alter {A} (f : option A -> option A) : positive -> pmap A -> pmap A :=
   alter_aux (ne_alter f) f.
+
+Definition ne_map {A B} (f : A -> B) : pmap_ne A -> pmap_ne B :=
+  fix go t :=
+    match t with
+    | PNode001 r => PNode001 (go r)
+    | PNode010 x => PNode010 (f x)
+    | PNode011 x r => PNode011 (f x) (go r)
+    | PNode100 l => PNode100 (go l)
+    | PNode101 l r => PNode101 (go l) (go r)
+    | PNode110 l x => PNode110 (go l) (f x)
+    | PNode111 l x r => PNode111 (go l) (f x) (go r)
+    end.
+
+Definition map {A B} (f : A -> B) (mt : pmap A) : pmap B :=
+  match mt with
+  | PEmpty => PEmpty
+  | PNodes t => PNodes (ne_map f t)
+  end.
+
+Definition filter_map_aux {A B} (go : pmap_ne A -> pmap B) (mt : pmap A) : pmap B :=
+  match mt with
+  | PEmpty => PEmpty
+  | PNodes t => go t
+  end.
+
+Definition ne_filter_map {A B} (f : A -> option B) : pmap_ne A -> pmap B :=
+  fix go t :=
+    pmap_ne_case t
+      (fun ml mx mr => PNode
+                         (filter_map_aux go ml)
+                         (option.bind mx f)
+                         (filter_map_aux go mr)).
+
+Definition filter_map {A B} (f : A -> option B) : pmap A -> pmap B :=
+  filter_map_aux (ne_filter_map f).
