shift-reset/var.v
@@ -1,4 +1,3 @@
 From Stdlib Require Import String.
 
-Inductive var : Type := Var : string -> var.
-Definition unvar (v : var) : string := match v with Var s => s end.
+Record var : Set := Var { var_car : string }.
